rebasing and fixing

case_study/lean/CaseStudy/Semantics/Definitions/Com_test.lean
@@ -35,7 +35,8 @@ def beval : BExp -> State -> Bool
   | BExp.and b_1 b_2, s => and (beval b_1 s) (beval b_2 s)
   | BExp.less n_1 n_2, s => (aeval n_1 s) < (aeval n_2 s)
 
-def state.update (name : String) (val : Int) (s : State) : State := λname' ↦ if name' = name then val else s name'
+def state.update (name : String) (val : Int) (s : State) : State := 
+  fun name' ↦ if name' = name then val else s name'
 
 -- some notations are stolen and adapted from LoVe lib others are stolen or inspired from https://github.com/leanprover-community/lean4-samples/blob/main/ListComprehension/README.md
 
@@ -59,12 +60,14 @@ inductive BigStep : Com × State -> State -> Prop where
     BigStep (Com.ite B S T, s) t
   | if_false (B S T s t) (hcond : ¬ (beval B s)) (hbody : BigStep (T, s) t) :
     BigStep (Com.ite B S T, s) t
-  | while_true (B S s t u) (hcond : beval B s) (hbody : BigStep (S, s) t) (hrest : BigStep (Com.while B S, t) u) :
+  | while_true (B S s t u) 
+    (hcond : beval B s) (hbody : BigStep (S, s) t) (hrest : BigStep (Com.while B S, t) u) :
     BigStep (Com.while B S, s) u
   | while_false (B S s) (hcond : ¬ beval B s) :
     BigStep (Com.while B S, s) s
 
-notation (name := big_step_judgement) prog_init_state_pair "==>" final_state => BigStep prog_init_state_pair final_state
+notation (name := big_step_judgement) 
+  prog_init_state_pair "==>" final_state => BigStep prog_init_state_pair final_state
 
 set_option quotPrecheck false
 notation (name := sem_equivalence) p "~" p' => forall s t, ((p, s) ==> t) <-> ((p', s) ==> t)
@@ -73,7 +76,8 @@ notation (name := sem_equivalence) p "~" p' => forall s t, ((p, s) ==> t) <-> ((
 inductive SmallStep : Com × State -> Com × State -> Prop where
   | var_assign (x a s) : SmallStep (x ::= a, s) (SKIP, s[x ↦ (aeval a s)])
   | seq_1 (c_2 s) : SmallStep (SKIP ;; c_2, s) (c_2, s)
-  | seq_2 (c_1 c_1' c_2 s s') : SmallStep (c_1 , s) (c_1', s') -> SmallStep (c_1 ;; c_2, s) (c_1' ;; c_2, s')
+  | seq_2 (c_1 c_1' c_2 s s') : 
+    SmallStep (c_1 , s) (c_1', s') -> SmallStep (c_1 ;; c_2, s) (c_1' ;; c_2, s')
   | if_true (b c_1 c_2 s) : beval b s -> SmallStep (IF b THEN c_1 ELSE c_2, s) (c_1, s)
   | if_false (b c_1 c_2 s) : ¬ (beval b s) -> SmallStep (IF b THEN c_1 ELSE c_2, s) (c_2, s)
   | while_loop (b c s) : SmallStep (WHILE b DO c, s) (IF b THEN c ;; WHILE b DO c ELSE SKIP, s)
@@ -89,7 +93,8 @@ theorem RTC_single {α : Type} {R : α → α → Prop} {a b : α} (hab : R a b)
   assumption
   apply RTC.refl
 
-theorem RTC_trans {α : Type} {R : α → α → Prop} {a b c : α} (hab : RTC R a b) (hbc : RTC R b c) : RTC R a c := by
+theorem RTC_trans {α : Type} {R : α → α → Prop} {a b c : α} (hab : RTC R a b) (hbc : RTC R b c) : 
+    RTC R a c := by
     induction hab with
       | refl => assumption
       | step _ _ _ _ _ ih =>
