case_study/lean/CaseStudy.lean
@@ -1,7 +1,12 @@
+import CaseStudy.Semantics.Definitions.Com
+import CaseStudy.Semantics.Definitions.Com_test
 import CaseStudy.Semantics.Base.Big_Step
 import CaseStudy.Semantics.Base.Small_Step
 import CaseStudy.Semantics.Hammered.Big_Step
 import CaseStudy.Semantics.Hammered.Big_Step_test
 import CaseStudy.Semantics.Hammered.Small_Step
+<<<<<<< HEAD
 import CaseStudy.Semantics.Definitions.Com
 import CaseStudy.Examples.MissingLemmas
+=======
+>>>>>>> 2061e22 (fixing imports)
